parallel_id

lambda.v
@@ -406,7 +406,7 @@ elim: t i s => /= [??? ni|t IH i ?|? IH1 ? IH2 ?? H].
 Qed.
 
 Definition s := 0.
-Definition t1 := Var 1.
+Definition t1 := Var 0.
 Definition t2 := (App (Abs (App (Var 0) (Var 0)))
                       (App (Abs (Var 0)) (Var 2))).
 Definition t := Var 0.
@@ -421,22 +421,50 @@ Compute max_var t1 <= i.
 Compute subst (subst t1 (s + i).+1 t) i (subst t2 s t) == subst (subst t1 i t2) (s + i) t.
 Compute vars (Abs (Abs t)).
 
-Lemma subst_subst t1 t2 s t i :
- max_var t1 < i ->
+Lemma parallel_id t s :
+  parallel t s -> parallel (App (Abs (Var 0)) t) s.
+Proof.
+elim: t s => [??|? IH ? /inf [] ? [] -> H|t IH1 ? IH2 ?].
+* rewrite /parallel mem_seq1 => /eqP ->.
+  by rewrite /parallel in_cons /= eqxx.
+* rewrite /parallel /= map_id !cats0 mem_cat; apply/orP; left.
+  by rewrite mem_map.
+* case: t IH1 => [??|??|???].
++ rewrite /parallel /= cats0 => /inf [] ? [] -> H.
+  rewrite map_id !cats0 !mem_cat; apply/orP; left.
+  by rewrite mem_map.
++ rewrite /parallel /= map_id !cats0 !mem_cat
+   => /orP [] /flatten_mapP [] ? p /inf []?[] -> ?.
+   apply/orP; left; apply/orP; left.
+   by apply/flatten_mapP/ex_intro2/subst_in.
+  apply/orP; left; apply/orP; right.
+  apply/flatten_mapP/ex_intro2; first by apply/p.
+  by rewrite mem_map.
++ rewrite /parallel /= !cats0 map_id mem_cat
+   => /flatten_mapP [] ? p /inf []?[] -> ?.
+  apply/orP; left.
+  apply/flatten_mapP/ex_intro2; first by apply/p.
+  by rewrite mem_map.
+Qed.
+
+Lemma subst_subst i t1 t2 s t :
+ max_var t1 <= i -> max_var t2 < s ->
  subst (subst t1 (s + i).+1 t) i (subst t2 s t) = subst (subst t1 i t2) (s + i) t.
 Proof.
-  elim: t1 t2 s t i => /= [????? H|t H ???? H0|? IH1 ? IH2 ???? H].
-  * case: ifP => [/eqP ni|].
-     rewrite ni addnC in H.
-     by move/ltnW/ltn_wl: H; rewrite ltnn.
-    rewrite ltnNge -addnS ltnW ?ltn_addl ?leqW //= subn0.
-    case: ifP => [/eqP ni|].
-     by rewrite ni ltnn in H.
-    rewrite ltnNge ltnW //= !subn0.
-    case: ifP => [/eqP ni|] //.
+  elim: t1 t2 s t i => /= [????? H|t H ???? H0 ?|? IH1 ? IH2 ???? H ?].
+  * case: ifP => [/eqP ni|_ H2].
      rewrite ni addnC in H.
      by move/ltn_wl: H; rewrite ltnn.
-    by rewrite ltnNge ltnW ?ltn_addl // subn0.
+    rewrite ltnNge -addnS ltnW ?ltn_addl //= subn0.
+    case: ifP => [/eqP ni|].
+     by rewrite !subst0 // ltn_addr.
+    rewrite ltnNge H !subn0 /=.
+    case: ifP => [/eqP ni ni'|].
+     move: ni ni' H => ->.
+     rewrite leq_eqVlt => -> /=.
+     rewrite addnC => /ltn_wl.
+     by rewrite ltnn.
+    by rewrite ltnNge (leq_trans H) ?leq_addl // subn0.
   * rewrite -addnS H //.
     by case: (max_var t) H0.
   * by rewrite ?(IH1, IH2, leq_trans _ H, ltnS, leq_maxr, leq_maxl).
@@ -448,7 +476,19 @@ Proof.
 move/parallelE => H /parallelE I; apply/parallelE.
 elim: I t t' s H => [?? -> */=|*/=|*/=|];try constructor;auto;first by case:ifP.
 move=> t1 t2 s1 s2 t1s1 IH1 t2s2 IH2 t t' s H.
-rewrite /=.
+case ms1 : (max_var s1 <= 0).
+ case ms2 : (max_var s2 < s).
+  move: (@subst_subst 0 _ _ _ t' ms1 ms2).
+  by rewrite addn0 => <-; constructor; auto.
+ move/negP/negP: ms2; rewrite -ltnNge ltnS.
+ case: t1 t1s1 ms1 IH1.
+ + move=> ? /parallelE.
+   rewrite /parallel mem_seq1 => /eqP ->.
+   rewrite /= leqn0 => /eqP -> /= _.
+  
+ rewrite /=.
+ rewrite /=.
+ 
 case: t1 t1s1 IH1.
 + move=> t1 /parallelE.
   rewrite /parallel mem_seq1 => /eqP -> /= IH1.
